Checkpoint

src/parse_formula.lean
@@ -1,4 +1,24 @@
-import .abel .fol
+import .abel .fol tactic
+
+/-
+namespace expr
+open format
+private meta def p := λ xs, paren (format.join (list.intersperse " " xs))
+
+meta def to_raw_fmt' {elab : bool} : expr elab → format
+| (var n) := p ["var", _root_.to_string n]
+| (sort l) := p ["sort", _root_.to_string l]
+| (const n ls) := p ["const", _root_.to_string n, _root_.to_string ls]
+| (mvar n m t)   := p ["mvar", _root_.to_string n, _root_.to_string m, to_raw_fmt t]
+| (local_const n m bi t) := p ["local_const", _root_.to_string n, _root_.to_string m, to_raw_fmt t]
+| (app e f) := p ["app", to_raw_fmt e, to_raw_fmt f]
+| (lam n bi e t) := p ["lam", _root_.to_string n, repr bi, to_raw_fmt e, to_raw_fmt t]
+| (pi n bi e t) := p ["pi", _root_.to_string n, repr bi, to_raw_fmt e, to_raw_fmt t]
+| (elet n g e f) := p ["elet", _root_.to_string n, to_raw_fmt g, to_raw_fmt e, to_raw_fmt f]
+| (macro d args) := sbracket (format.join (list.intersperse " " ("macro" :: _root_.to_string (macro_def_name d) :: args.map to_raw_fmt)))
+
+end expr
+-/
 
 universe u
 
@@ -14,19 +34,22 @@ meta def to_fmla : pexpr → option fmla
 
 namespace tactic
 namespace interactive
+
+section parse_formula
 open interactive interactive.types expr
 
 meta def parse_formula (e : parse texpr) : tactic unit :=
 do f <- to_fmla e, tactic.exact `(f)
 
+end parse_formula
 end interactive
 end tactic
 
 def foo : fmla := by parse_formula (∀ x : ℕ, x)
-#print foo -- fmla.pi (fmla.var 0)
+-- #print foo -- fmla.pi (fmla.var 0)
 
--- meta def my_dumb_reflect (n : ℕ) : tactic unit :=
--- tactic.exact (reflect (n+1))
+meta def my_dumb_reflect (n : ℕ) : tactic unit :=
+tactic.exact (reflect (n+1))
 
 -- meta def my_dumber_reflect (n : ℕ) : tactic unit :=
 -- tactic.trace `n
@@ -36,8 +59,6 @@ def foo : fmla := by parse_formula (∀ x : ℕ, x)
 -- run_cmd my_dumber_reflect 500 -- n
 
 -- def foo' : ℕ := by my_dumber_reflect 500
-
-
 
 -- meta def my_dumber_reflect' (x : ℕ) : tactic unit :=
 -- tactic.exact `(n + 1)
@@ -71,12 +92,13 @@ meta def to_term : Π {n : ℕ}, pexpr → option (preterm L_abel n)
 
 end abel_parse_formula
 
+section weekdays
 @[derive has_reflect]
 inductive weekday : Type
 | monday          : weekday
 | another_day     : weekday → weekday
 
-export weekday
+open weekday
 
 meta def dump_weekday (f : weekday) : tactic unit :=
 tactic.trace $ to_string (expr.to_raw_fmt (reflect f).to_expr) 
@@ -88,7 +110,7 @@ inductive weekday' : Type
 | monday          : weekday'
 | another_day     : weekday' → weekday'
 
-export weekday'
+open weekday'
 meta instance has_reflect_weekday' : has_reflect weekday'
 | weekday'.monday                  := `(monday)
 | (weekday'.another_day x)         := `(λ l, weekday'.another_day l).subst $
@@ -100,43 +122,109 @@ tactic.trace $ to_string (expr.to_raw_fmt (reflect f).to_expr)
 
 run_cmd dump_weekday' (another_day (another_day monday))
 -- (app (const weekday'.another_day []) (app (const weekday'.another_day []) (const weekday'.monday [])))
-
+end weekdays
 -- meta instance has_reflect_preterm {L : Language.{u}} : Π{n : ℕ}, has_reflect (preterm L n)
--- | 0 (var k) := `(λ y, preterm.var y).subst `(reflect k)
+-- | 0 (var k) := `(λ y, preterm.var y).subst begin end
+
+-- @[derive has_reflect]
+
+section preterm_aux 
+inductive preterm_aux (L : Language.{u}) : Type u
+| var     : ℕ → preterm_aux
+| func    : ∀ k : ℕ, L.functions k → preterm_aux
+| app     : preterm_aux → preterm_aux → preterm_aux
+
+def to_aux {L : Language.{u}} : ∀ {l : ℕ},  preterm L l → preterm_aux L
+| 0 (var n)      := preterm_aux.var _ n
+| k (func f)     := preterm_aux.func _ f
+| k (app t₁ t₂)  := preterm_aux.app (to_aux t₁) (to_aux t₂)
 
 
 def L_abel_plus' (t₁ t₂ : preterm L_abel 0) : preterm L_abel 0 :=
 @term_of_function L_abel 2 (abel_functions.plus : L_abel.functions 2) t₁ t₂
+end preterm_aux
 
 local infix ` +' `:100 := L_abel_plus'
 
 local notation ` zero ` := (func abel_functions.zero : preterm L_abel 0)
-meta def str_preterm : ∀ n : ℕ, ℕ → preterm L_abel n → string
- | n z &k := "x" ++ to_string(z - k)
- | n z (func abel_functions.zero) := "0"
- | n z (func abel_functions.plus) := "+"
- | n z (app t₁ t₂) := (str_preterm _ z t₁) ++ "(" ++ (str_preterm _ z  t₂) ++ ")"
 
-#eval str_preterm _ 4 (zero +' zero)
+section L_abel_term_biopsy
+
+def sample1 : preterm L_abel 0 := (zero +' zero)
+
+def sample2 : preterm L_abel 0 := zero
+
+-- #reduce sample2
+
+open expr
+meta def sample2_expr : expr :=
+mk_app (const `preterm.func list.nil) ([(const `L_abel list.nil), `(0), const `abel_functions.zero list.nil] : list expr)
+
+-- begin
+--   refine app _ _,
+--   exact const `preterm.func list.nil,
+--   exact const `abel_functions.zero list.nil
+-- end
+
+-- #check mk_app
+
+-- #print preterm.func
+
+-- #eval (to_raw_fmt sample2_expr).to_string
+
+-- def sample2_again : preterm L_abel 0 :=
+-- by tactic.exact sample2_expr -- unknown declaration preterm.func
+
+end L_abel_term_biopsy
+
+section simpler_biopsy
+
+inductive my_inductive : Type
+| a : my_inductive
+| b : my_inductive
+| f : my_inductive → my_inductive
+
+open my_inductive
+def sample3 : my_inductive := f a
+
+open expr
+
+meta def sample3_expr : expr :=
+app (const `my_inductive.f list.nil) (const `my_inductive.a list.nil)
+
+def sample3_again : my_inductive := by tactic.exact (sample3_expr)
+
+example : sample3 = sample3_again := rfl
+
+end simpler_biopsy
+
+
+ 
+-- meta def str_preterm : ∀ n : ℕ, ℕ → preterm L_abel n → string
+--  | n z &k := "x" ++ to_string(z - k)
+--  | n z (func abel_functions.zero) := "0"
+--  | n z (func abel_functions.plus) := "+"
+--  | n z (app t₁ t₂) := (str_preterm _ z t₁) ++ "(" ++ (str_preterm _ z  t₂) ++ ")"
+
+-- #eval str_preterm _ 4 (zero +' zero)
 
 namespace tactic
 namespace interactive
 open interactive interactive.types expr
 
-#check format
-
 def my_test_term : preterm L_abel 0 := (zero +' zero)
 
-@[instance]meta def format_preterm {n} : has_to_tactic_format (preterm L_abel n) :=
-{ to_tactic_format := λ t, return ((str_preterm _ 0 t)) }
+-- @[instance]meta def format_preterm {n} : has_to_tactic_format (preterm L_abel n) :=
+-- { to_tactic_format := λ t, return ((str_preterm _ 0 t)) }
 
-meta def parse_term (n : ℕ) (e : parse texpr) : tactic unit :=
+meta def parse_term -- (n : ℕ) (e : parse texpr)
+: tactic unit :=
 do trace "hello"
 
-example : false :=
-begin
-  parse_term 0 (&0 : preterm L_abel 0)
-end
+-- example : false :=
+-- begin
+--   parse_term, sorry
+-- end
 
 -- def my_dumb_term : preterm L_abel 0 := by parse_term 0 (abel_functions.zero)
 
@@ -144,8 +232,24 @@ end interactive
 end tactic
 
 section test
-def my_term : preterm L_abel 0 := sorry
+-- def my_term : preterm L_abel 0 := sorry
 
-#check tactic.interactive.rcases
+-- #check tactic.interactive.rcases
 
 end test
+
+
+section sample4
+
+/-- Note: this is the same as `dfin` -/
+inductive my_indexed_family : ℕ → Type u
+| z {} : my_indexed_family 0
+| s : ∀ {k}, my_indexed_family k → my_indexed_family (k+1)
+
+open my_indexed_family
+
+def sample4 : my_indexed_family 1 := s z
+
+-- #check tactic.eval_expr
+
+end sample4
